updating the bonus homework

teaching/taltech2020/ex/hw/FileSystem.fst
@@ -5,19 +5,19 @@ module FileSystem
   Homework exercise.
 
   In this exercise you are asked to implement an FStar-version of the 
-  small file system from your regular coursework. This exercise differs 
-  from your regular coursework in that we will not use randomised testing 
-  to check the correctness of your implementation, but instead you are 
-  asked to equip the `show`, `create_dir`, and `delete` functions with 
-  strong specifications and prove that your implementations satisfy them.
+  small file system from your coursework no. 7. This exercise differs 
+  from your regular coursework in that we will not use randomised 
+  testing to check the correctness of your implementation, but instead 
+  you are asked to equip the `create` and `delete` functions with strong
+  specifications, and prove that your implementations satisfy them.
 
   The exercise is divided into 7 tasks---see below for further details. 
   The tasks are somewhat independent. For instance, you can either first
   implement the file system operations (Tasks 4-6) and then strengthen 
   their specifications (Task 7); or you can first try to come up with 
   suitably strong specifications for them to verify `FileSystemClient.fst`
-  (Task 7) and only afterwards try to come up with real implementations 
-  that would also satisfy these stronger specifications.
+  (Task 7), and only afterwards try to come up with the actual 
+  implementations that would satisfy these stronger specifications.
 
   When solving the tasks below, do not be afraid of defining additional 
   auxiliary (pure) recursive functions, state and prove lemmas about 
@@ -28,64 +28,264 @@ module FileSystem
 open FStar.List.Tot // FStar's lists library which could be useful below
 open FStar.Classical // FStar's classical logic library which could also be useful below
 
-(* 
 
-  Task 1: Define the type of well-formed paths as lists of strings (i.e., 
-          raw paths) that do not contain nodes with empty names. In other 
-          words, replace `admit` in the definition of `path_wf` with a 
-          predicate on path `p` that ensures its well-formedness. That 
-          you got well-formedness right will be tested with the auxiliary 
-          lemmas `test_wf_path` and `test_not_wf_path` on example paths.
-          
+(*
+
+   The raw file system and raw paths in it are defined exactly as in your 
+   regular coursework: raw paths are lists of strings, and the type of 
+   raw file systems is a recursively defined tree-like record datatype.
+   
 *)
 
-let path_wf (p:list string) : Type0 = 
-  admit ()
+type path = list string
 
-type path = p:list string{path_wf p}
+type fstree = { name:string ;
+                children:list fstree }
 
-let test_wf_path () : Lemma (path_wf ("home" :: "username" :: [])) = 
-  ()
+let mk_fstree (name:string) (children:list fstree) =
+  { name = name; children = children }
 
-let test_not_wf_path () : Lemma (~(path_wf ("home" :: "" :: "username" :: []))) = 
-  ()
 
-(* Type of file systems *)
-
-type fs_tree =
-  | Node : list (string * fs_tree) -> fs_tree
 
 (* 
 
-  Task 2: Define a well-formedness predicate for file systems (replace the admit 
-          with in `fs_tree_wf` actual code). As in your regular coursework, a 
-          file system is well-formed when identical paths cannot lead to different 
-          nodes in the tree, and a well-formed file system also should not have 
-          nodes with empty names. That you got well-formedness right will be tested 
-          below with the auxiliary lemmas `test_wf_fs` and `test_not_wf_fs`.
+  Task 1: Define the type `wf_path` of well-formed paths as raw paths that:
+
+          - do not contain nodes with empty names; and 
+
+          - are nonempty (this is a stronger condition than required by the
+            `pathWf` predicate in your regular coursework, but it will make 
+            defining the file system operations below more convenient). 
+                    
+          In other words, replace the `admit` in `path_wf` with a (bool-valued) 
+          predicate on the path `p` that ensures this kind of well-formedness.
           
 *)
 
-assume val sub_dir_smaller (s:string) (fs:fs_tree) (ns:list (string * fs_tree)) // This is to help the typechecker know that
-  : Lemma (Node ns << Node ((s,fs) :: ns))                                      // subdirectories in the tree have smaller size
-    [SMTPat (Node ((s,fs) :: ns))]
+let rec path_wf (p:path) : bool = 
+  admit ()
+  
+type wf_path = p:path{path_wf p}
 
-let rec fs_tree_wf (fs:fs_tree) : Type0 = 
+
+(*
+
+  Sanity checking that you got the well-formedness of raw paths correct. 
+  
+*)
+
+let check_wf_path () : Lemma (path_wf ("home" :: "username" :: [])) = 
+  ()
+
+let check_not_wf_path () : Lemma (~(path_wf ("home" :: "" :: "username" :: []))) = 
+  ()
+
+
+
+(* 
+
+  Task 2: Define the type `wf_fstree` of well-formed file systems as a refinement 
+          of raw file systems. That is, replace the `admit` in `fstree_wf` with a 
+          predicate which ensures that in the given file system `fs`:
+          
+          - the path to any directory in the file system is well-formed; and
+            
+          - the file system is deterministic (for any given path, there is at most 
+            one directory in the file system with that path.
+            
+*)
+
+let rec fstree_wf (fs:fstree) : bool = 
   admit ()
 
-let wf_fs_tree = fs:fs_tree{fs_tree_wf fs}
+let wf_fstree = fs:fstree{fstree_wf fs}
 
-let test_wf_fs () : Lemma (fs_tree_wf (Node (("home",Node (("username",Node []) :: [])) :: []))) = 
+
+(* 
+
+  Sanity checking that you got the well-formedness of raw file systems correct. 
+  
+*)
+
+let check_wf_fs () 
+  : Lemma (fstree_wf (
+      mk_fstree "/"
+        [
+        mk_fstree "home"
+        [ 
+          mk_fstree "username1" 
+          [
+            mk_fstree "documents" [];
+            mk_fstree "downloads" [];            
+          ];
+          mk_fstree "username2" 
+          [
+            mk_fstree "documents" []
+          ]
+        ]
+        ])) = 
   ()
 
-let test_not_wf_fs () : Lemma (~(fs_tree_wf (Node (("home",Node (("",Node (("username",Node []) :: [])) :: [])) :: 
-                                                   ("home",Node []) :: 
-                                                   ("home",Node []) :: [])))) = 
+let check_not_wf_fs_path () 
+  : Lemma (not (fstree_wf (
+      mk_fstree "/"
+        [
+        mk_fstree "home"
+        [ 
+          mk_fstree "username1" 
+          [
+            mk_fstree "documents" [];
+            mk_fstree "downloads" [];            
+          ];
+          mk_fstree "" 
+          [
+            mk_fstree "documents" []
+          ]
+        ]
+        ]))) =
   ()
 
-(* A (monadic) effect that characterises programs that use a file system. *)
+let check_not_wf_fs_nondet () 
+  : Lemma (not (fstree_wf (
+      mk_fstree "/"
+        [
+        mk_fstree "home"
+        [ 
+          mk_fstree "username" 
+          [
+            mk_fstree "documents" [];
+            mk_fstree "downloads" [];            
+          ];
+          mk_fstree "username" 
+          [
+            mk_fstree "documents" []
+          ]
+        ]
+        ]))) =
+  ()
 
-let fs_st (a:Type) = fs_tree -> M (a * fs_tree)
+
+
+(*
+
+  Task 3: Define a predicate on (raw) file systems  that holds if a  
+          given well-formed path exists in a given (raw) file system.
+
+          For convenience, we use the convention here that the path `p` 
+          is given relative to the root directory (but **does not** 
+          contain the root). So, if the root of a file system `fs` is "/", 
+          then `in_fstree ["home"; "username"] fs` holds if the file
+          system `fs` includes the path `["/"; "home"; "username"]`.
+          
+*)
+
+let rec in_fstree (p:wf_path) (fs:fstree) : bool = 
+  admit ()
+
+
+
+(* 
+
+  Sanity checking that you got the path inclusion predicate correct. 
+  
+*)
+
+let check_in_fstree1 ()
+  : Lemma (["home"; "username1"; "downloads"]
+           `in_fstree`
+           mk_fstree "/"
+             [
+             mk_fstree "home"
+             [
+               mk_fstree "username1" 
+               [
+                 mk_fstree "documents" [];
+                 mk_fstree "downloads" [];            
+               ];
+               mk_fstree "username2" 
+               [
+                 mk_fstree "documents" []
+               ]
+             ]
+           ]) =
+  ()
+
+let check_in_fstree2 ()
+  : Lemma (["home"; "username2"] 
+           `in_fstree`
+           mk_fstree "/"
+             [
+             mk_fstree "home"
+             [
+               mk_fstree "username1" 
+               [
+                 mk_fstree "documents" [];
+                 mk_fstree "downloads" [];            
+               ];
+               mk_fstree "username2" 
+               [
+                 mk_fstree "documents" []
+               ]
+             ]
+           ]) =
+  ()
+
+let check_not_in_fstree ()
+  : Lemma (not (["home"; "username3"; "downloads"]
+                `in_fstree`
+                mk_fstree "/"
+                  [
+                  mk_fstree "home"
+                  [
+                    mk_fstree "username1" 
+                    [
+                      mk_fstree "documents" [];
+                      mk_fstree "downloads" [];            
+                    ];
+                    mk_fstree "username2" 
+                    [
+                      mk_fstree "documents" []
+                    ]
+                  ]
+                ])) =
+  ()
+
+
+
+(*
+
+  Task 4: Prove that if a path is included in a given file system,
+          then any prefix of this path is also in that file system.
+
+          These lemmas and the SMT patterns attached to them will
+          help us to automatically deduce that if `["a"; "b"; "c"]`
+          is a well-formed path, then so are `["a"]` and `["a"; "b"]`, 
+          and similarly for the containment of prefixes in file systems.
+
+*)
+
+let rec lemma_path_wf_append (p q:path)
+  : Lemma (requires (path_wf p /\ path_wf q))
+          (ensures  (path_wf (append p q)))
+          [SMTPat (path_wf (append p q))] =
+  admit ()
+
+let rec lemma_in_fstree_append (p q:wf_path) (fs:fstree)
+  : Lemma (requires (append p q `in_fstree` fs))
+          (ensures  (p `in_fstree` fs))
+          [SMTPat (append p q `in_fstree` fs); 
+           SMTPat (p `in_fstree` fs)] = 
+  admit ()
+
+
+
+(*
+
+  A (monadic) effect that characterises programs that use a file system. 
+  
+*)
+
+let fs_st (a:Type) = fstree -> M (a * fstree)
 
 let return_fs_st (a:Type) (x:a) : fs_st a 
   = fun fs0 -> (x,fs0)
@@ -94,10 +294,10 @@ let bind_fs_st (a:Type) (b:Type) (f:fs_st a) (g:a -> fs_st b) : fs_st b
   = fun fs0 -> let (x,fs1) = f fs0 in 
               g x fs1
 
-let read_st () : fs_st fs_tree 
+let read_st () : fs_st fstree 
   = fun fs0 -> (fs0,fs0)
 
-let write_st (fs:fs_tree) : fs_st unit 
+let write_st (fs:fstree) : fs_st unit 
   = fun _ -> ((), fs)
 
 total new_effect {
@@ -109,92 +309,99 @@ total new_effect {
      ; write    = write_st
 }
 
-(* Pre- and postcondition variant of the `FileSystem` effect, which additionally 
-   assumes that the initial file system (`fs0`) is well-formed and additionally 
-   requires one to prove that the final file system (`fs1`) remains well-formed. *)
+
+(* 
+
+  A pre- and postcondition variant of the `FileSystem` effect, which additionally 
+  assumes that the initial file system (`fs0`) is well-formed and additionally 
+  requires one to prove that the final file system (`fs1`) remains well-formed. 
+   
+*)
 
 effect FS (a:Type) 
-          (pre:wf_fs_tree -> Type0) 
-          (post:wf_fs_tree -> a -> wf_fs_tree -> Type0) = 
+          (pre:wf_fstree -> Type0) 
+          (post:wf_fstree -> a -> wf_fstree -> Type0) = 
   FileSystem a (fun fs0 p -> 
-                 fs_tree_wf fs0 /\ 
+                 fstree_wf fs0 /\ 
                  pre fs0 /\ 
-                 (forall x fs1 . (post fs0 x fs1 /\ fs_tree_wf fs1) ==> p (x,fs1)))
+                 (forall x fs1 . (post fs0 x fs1 /\ fstree_wf fs1) ==> p (x,fs1)))
 
-(* Effectful actions to read and update the file system in your code below. *)
 
-let read (_:unit) : FS wf_fs_tree
+(* 
+
+  Effectful actions to read and update the file system in your code below. 
+  
+*)
+
+let read (_:unit) : FS wf_fstree
                        (requires (fun _ -> True)) 
                        (ensures  (fun fs0 fs fs1 -> fs0 == fs /\ fs == fs1)) = 
   FileSystem?.read ()
 
-let write (fs:wf_fs_tree) : FS unit 
-                               (requires (fun _ -> True)) 
-                               (ensures  (fun _ _ fs1 -> fs1 == fs)) = 
+let write (fs:wf_fstree) : FS unit 
+                              (requires (fun _ -> True)) 
+                              (ensures  (fun _ _ fs1 -> fs1 == fs)) = 
   FileSystem?.write fs
+  
+
+
+(* 
+
+  Task 5: Define a function in the `FS` effect that creates a new directory in the 
+          file system. If the directory exists, then keep the file system as is.
+
+          For convenience, we use the convention here that the path `p` is given
+          relative to the root directory (but **does not** contain the root). So, if
+          the root of a file system `fs` is "/", then `create ["home"; "username"] fs`
+          would create a new directory at path `["/"; "home"; "username"]` in `fs`.
+
+  Hint: As part of defining `create`, you need to prove that creating a well-formed
+        path in a well-formed file system results in a well-formed file system. 
+        
+*)
+
+let create (p:wf_path) : FS unit 
+                            (requires (fun fs0 -> True)) 
+                            (ensures  (fun fs0 _ fs1 -> True)) = 
+  admit ()
+
+
 
 (*
 
-   Task 3: Define a predicate that holds if a given path exists in a given file system.
-
-*)
-
-let in_fs (p:path) (fs:wf_fs_tree) : Type0 = 
-  admit ()
-
-(* 
-
-  Task 4: Define a function in the the `FS` effect that returns all paths in the file system.
-        
-*)
-           
-let show () : FS (list path)
-                 (requires (fun fs0 -> True)) 
-                 (ensures  (fun fs0 ps fs1 -> True)) =
-  admit ()
-
-(* 
-
-  Task 5: Define a function in the `FS` effect that creates a new directory in the file system. 
-
-  Hint: As part of defining `create_dir`, you also need to prove that creating a well-formed 
-        path in a well-formed tree results in a well-formed tree. 
-        
-*)
-
-let create_dir (p:path) : FS unit 
-                             (requires (fun fs0 -> True)) 
-                             (ensures  (fun fs0 _ fs1 -> True)) = 
-  admit ()
-
-(* 
-
   Task 6: Define a function in the `FS` effect that deletes a given path from the file system. 
+
+          For convenience, we again use the convention here that the path `p` is given
+          relative to the root directory (but **does not** contain the root). So, if
+          the root of a file system `fs` is "/", then `delete ["home"; "username"] `fs``
+          would delete the directory at path `["/"; "home"; "username"]` in `fs`.
 
   Hint: As part of defining `delete`, you also need to prove that deleting a well-formed path 
         from a well-formed tree results in a well-formed tree. 
 
 *)
 
-let delete (p:path) : FS unit
-                         (requires (fun fs0 -> True))
-                         (ensures  (fun fs0 _ fs1 -> True)) =
+let delete (p:wf_path) : FS unit
+                            (requires (fun fs0 -> True))
+                            (ensures  (fun fs0 _ fs1 -> True)) =
   admit ()
+
+
 
 (* 
 
-  Task 7: Strengthen the (currently trivial) specifications of `show`, `create_dir`, and
-          `delete` so that the test code in `FileSystemClient.fst` successfully typechecks. 
+  Task 7: Strengthen the (currently trivial) specifications of `create` and `delete`
+          so that the test code in `FileSystemClient.fst` successfully typechecks. 
                
-  Hint 1: Think about the resulting shape of the file system after creating a new path in it or 
-          removing an already existing path. You can draw inspiration from the `deleteDeletes`
-          and `createAndDelete` FSCheck properties you defined in your regular coursework. 
-          Similarly, the list of paths returned by `show` is not any old list of paths. 
+  Hint 1: Think about the resulting shape of the file system after creating a new path
+          in it or removing an already existing path. You can draw inspiration from the 
+          `deleteDeletes` and `createAndDelete` FSCheck properties you defined in your 
+          regular coursework. 
 
-  Hint 2: Do not be afraid of defining auxiliary pure functions (using the default `Tot` effect)
-          which you can then use as part of the specifications. Most probably you will also
-          need to state and prove some lemmas about these functions (using the `Lemma` effect), 
-          e.g., so as to relate the spec of `create_dir` to the spec of `delete` if one follows 
-          the other in user code (as in FileSystemClient.fst).
+  Hint 2: Do not be afraid of defining auxiliary pure functions (using the default `Tot` 
+          effect) which you can then use as part of the specifications. Most probably
+          you will also need to state and prove some lemmas about these functions (using 
+          the `Lemma` effect), e.g., so as to relate the spec of `create` to the spec of 
+          `delete` if one follows the other in user code (as in FileSystemClient.fst).
 
 *)
