teaching/taltech2020/ex/hw/FileSystemClient.fst
@@ -11,67 +11,82 @@ module FileSystemClient
 
 *)
 
-open FileSystem
-
 open FStar.List.Tot
 
-//[@expect_failure]
-let test1 (p:path) : FS unit 
-                        (requires (fun fs0 -> fs0 == Node []))
-                        (ensures  (fun fs0 _ fs1 -> fs0 == fs1)) =
-  create_dir p;
+open FileSystem
+
+//[@(expect_failure)]
+let test0 (p:wf_path) : FS unit
+                           (requires (fun fs0 -> (["home"] @ ["username"]) `in_fstree` fs0))
+                           (ensures  (fun _ _ fs1 -> ["home"] `in_fstree` fs1)) =
+  ()
+
+//[@(expect_failure)]
+let test1 (p:wf_path) : FS unit
+                           (requires (fun fs0 -> True))
+                           (ensures  (fun _ _ fs1 -> p `in_fstree` fs1)) =
+  create p
+
+//[@(expect_failure)]
+let test2 (p:wf_path) : FS unit
+                           (requires (fun fs0 -> True))
+                           (ensures  (fun _ _ fs1 -> not (p `in_fstree` fs1))) =
   delete p
 
-//[@expect_failure]
-let test2 (p:path) : FS unit
-                        (requires (fun fs0 -> fs0 == Node []))
-                        (ensures  (fun fs0 _ fs1 -> fs0 == fs1)) =
-  create_dir p;
-  let _ = show () in
-  delete p
+//[@(expect_failure)]
+let test3 (p q:wf_path) : FS unit
+                             (requires (fun fs0 -> p `in_fstree` fs0))
+                             (ensures  (fun _ _ fs1 -> p `in_fstree` fs1 /\ q `in_fstree` fs1)) =
+  create q
 
-//[@expect_failure]
-let test3 (p:path) : FS unit
-                        (requires (fun fs0 -> True))
-                        (ensures  (fun fs0 _ fs1 -> in_fs p fs1)) =
-  create_dir p
+//[@(expect_failure)]
+let test4 (p q r:wf_path) : FS unit
+                             (requires (fun fs0 -> p `in_fstree` fs0))
+                             (ensures  (fun _ _ fs1 -> p `in_fstree` fs1 /\ q `in_fstree` fs1 /\ r `in_fstree` fs1)) =
+  create q;
+  create r
 
-//[@expect_failure]
-let test4 (p:path) : FS unit
-                        (requires (fun fs0 -> True))
-                        (ensures  (fun fs0 _ fs1 -> ~(in_fs p fs1))) =
-  delete p
+//[@(expect_failure)]
+let test5 () : FS unit
+                  (requires (fun fs0 -> (["home"] @ ["username1"]) `in_fstree` fs0))
+                  (ensures  (fun _ _ fs1 -> (["home"] @ ["username1"]) `in_fstree` fs1)) =
+  delete ["home"; "username2"]
 
-//[@expect_failure]
-let test5 (p:path) : FS (list path)
-                        (requires (fun fs0 -> fs0 == Node []))
-                        (ensures  (fun fs0 ps fs1 -> mem p ps /\ fs0 == fs1)) =
-  create_dir p;
-  let ps = show () in
-  delete p;
-  ps
+//[@(expect_failure)]
+let test6 () : FS unit
+                  (requires (fun fs0 -> (["home"] @ ["username"] @ ["documents"]) `in_fstree` fs0 /\
+                                     (["home"] @ ["username"] @ ["downloads"]) `in_fstree` fs0))
+                  (ensures  (fun _ _ fs1 -> not ((["home"] @ ["username"] @ ["documents"]) `in_fstree` fs1) /\
+                                         not ((["home"] @ ["username"] @ ["downloads"]) `in_fstree` fs1))) =
+  delete (["home"] @ ["username"])
 
-//[@expect_failure]
-let test6 (p1 p2 p3:path) : FS unit 
-                               (requires (fun fs0 -> fs0 == Node []))
-                               (ensures  (fun fs0 _ fs1 -> fs0 == fs1)) =
-  create_dir p1;
-  create_dir p2;
-  delete p1;
-  create_dir p3;
-  delete p2;
-  delete p3
 
-//[@expect_failure]
-let test7 (p1 p2:path) : FS unit
-                        (requires (fun fs0 -> True))
-                        (ensures  (fun _ _ fs1 -> in_fs p1 fs1 /\ in_fs p2 fs1)) =
-  create_dir p1;
-  create_dir p2
+//[@(expect_failure)]
+let test7 () : FS unit
+                  (requires (fun fs0 -> (["home"] @ ["username1"]) `in_fstree` fs0 /\
+                                     (["home"] @ ["username2"] @ ["documents"]) `in_fstree` fs0 /\
+                                     (["home"] @ ["username3"]) `in_fstree` fs0))
+                  (ensures  (fun _ _ fs1 -> (["home"] @ ["username2"] @ ["documents"]) `in_fstree` fs1)) =
+  delete (["home"] @ ["username1"]);
+  delete (["home"] @ ["username3"])
 
-//[@expect_failure]
-let test8 (p1 p2:path) : FS unit
-                            (requires (fun fs0 -> True))
-                            (ensures  (fun _ _ fs1 -> ~(in_fs p1 fs1) /\ ~(in_fs p2 fs1))) =
-  delete p1;
-  delete p2
+//[@(expect_failure)]
+let test8 (p:wf_path) : FS unit
+                           (requires (fun fs0 -> True))
+                           (ensures  (fun _ _ fs1 -> not ((["home"] @ ["username"]) `in_fstree` fs1))) =
+  create (["home"] @ ["username"]);
+  delete (["home"] @ ["username"])
+
+//[@(expect_failure)]
+let test9 (p:wf_path) : FS unit
+                           (requires (fun fs0 -> True))
+                           (ensures  (fun _ _ fs1 -> (["home"] @ ["username2"] @ ["downloads"]) `in_fstree` fs1 /\
+                                                  not ((["home"] @ ["username1"] @ ["documents"]) `in_fstree` fs1) /\
+                                                  not ((["home"] @ ["username1"]) `in_fstree` fs1) /\
+                                                  (["home"] @ ["username3"]) `in_fstree` fs1)) =
+  create (["home"] @ ["username1"]);
+  create (["home"] @ ["username2"]);
+  create (["home"] @ ["username1"] @ ["documents"]);
+  create (["home"] @ ["username2"] @ ["downloads"]);
+  delete (["home"] @ ["username1"]);
+  create (["home"] @ ["username3"])
